Proved the root always exists for LstGraph.

sample_mark/verif_unionfind.v
@@ -23,6 +23,7 @@ Local Identity Coercion SGraph_SpatialGraph: SGraph >-> SpatialGraph.
 Local Coercion pg_lg: LabeledGraph >-> PreGraph.
 
 Notation vertices_at sh P g:= (@vertices_at _ _ _ _ _ _ (@SGP pSGG_VST nat unit (sSGG_VST sh)) _ P g).
+Notation whole_graph sh g := (vertices_at sh (vvalid g) g).
 Notation graph sh x g := (@reachable_vertices_at _ _ _ _ _ _ _ _ _ _ (@SGP pSGG_VST nat unit (sSGG_VST sh)) _ x g).
 Notation Graph := (@Graph pSGG_VST nat unit unit).
 Existing Instances maGraph finGraph liGraph RGF.
@@ -47,25 +48,25 @@ Definition find_spec :=
   PRE [ _x OF (tptr (Tstruct _Node noattr))]
           PROP  (vvalid g x)
           LOCAL (temp _x (pointer_val_val x))
-          SEP   (graph sh x g)
+          SEP   (whole_graph sh g)
   POST [ tptr (Tstruct _Node noattr) ]
         EX g': Graph, EX rt : pointer_val,
         PROP (findS g x g' /\ uf_root g' x rt)
         LOCAL (temp ret_temp (pointer_val_val rt))
-        SEP (vertices_at sh (reachable g x) g').
+        SEP (whole_graph sh g').
 
 Definition unionS_spec :=
  DECLARE _unionS
   WITH sh: wshare, g: Graph, x: pointer_val, y: pointer_val
   PRE [ _x OF (tptr (Tstruct _Node noattr)), _y OF (tptr (Tstruct _Node noattr))]
-          PROP  (weak_valid g x /\ weak_valid g y)
+          PROP  (vvalid g x /\ vvalid g y)
           LOCAL (temp _x (pointer_val_val x); temp _y (pointer_val_val y))
-          SEP   (graph sh x g * graph sh y g)
+          SEP   (whole_graph sh g)
   POST [ Tvoid ]
         EX g': Graph,
         PROP (uf_union g x y g')
         LOCAL()
-        SEP (graph sh x g').
+        SEP (whole_graph sh g').
 
 (*
 Definition makeSet_spec :=
@@ -128,6 +129,24 @@ Proof.
         } rewrite H3. entailer !.
 Qed.
 
+Lemma false_Cne_eq: forall x y, typed_false tint (force_val (sem_cmp_pp Cne (pointer_val_val x) (pointer_val_val y))) -> x = y.
+Proof.
+  intros. hnf in H. destruct x, y; inversion H; auto. simpl in H. clear H1. unfold sem_cmp_pp in H. simpl in H. destruct (eq_block b b0).
+  - destruct (Int.eq i i0) eqn:? .
+    + symmetry in Heqb1. apply binop_lemmas2.int_eq_true in Heqb1. subst; auto.
+    + simpl in H. inversion H.
+  - simpl in H. inversion H.
+Qed.
+
+Lemma true_Cne_neq: forall x y, typed_true tint (force_val (sem_cmp_pp Cne (pointer_val_val x) (pointer_val_val y))) -> x <> y.
+Proof.
+  intros. hnf in H. destruct x, y; inversion H; [|intro; inversion H0..]. simpl in H. clear H1. unfold sem_cmp_pp in H. simpl in H. destruct (eq_block b b0).
+  - destruct (Int.eq i i0) eqn:? .
+    + simpl in H. inversion H.
+    + subst b0. apply int_eq_false_e in Heqb1. intro. inversion H0. auto.
+  - intro. inversion H0. auto.
+Qed.
+
 Lemma body_find: semax_body Vprog Gprog f_find find_spec.
 Proof.
   start_function.
@@ -145,77 +164,32 @@ Proof.
   unlocalize
     (PROP  ()
      LOCAL (temp _p (pointer_val_val pa); temp _x (pointer_val_val x))
-     SEP  (graph sh x g)).
+     SEP  (whole_graph sh g)).
   Grab Existential Variables.
   Focus 2. {
     simplify_ramif. rewrite <- H0. simpl.
-    apply (@va_reachable_root_stable_ramify _ _ _ _ SGBA_VST _ _ _ _ _ _ (SGA_VST sh) g x (r, pa)); auto.
+    apply (@vertices_at_ramif_1_stable _ _ _ _ SGBA_VST _ _ (SGA_VST sh) g (vvalid g) x (r, pa)); auto.
   } Unfocus.
   unfold semax_ram.
   forward_if_tac
     (EX g': Graph, EX rt : pointer_val,
      PROP (findS g x g' /\ uf_root g' x rt)
      LOCAL (temp _p (pointer_val_val rt); temp _x (pointer_val_val x))
-     SEP (vertices_at sh (reachable g x) g'));
+     SEP (whole_graph sh g'));
     [apply ADMIT | | gather_current_goal_with_evar ..].
-  localize
-    (PROP (vvalid g pa)
-     LOCAL (temp _p (pointer_val_val pa); temp _x (pointer_val_val x))
-     SEP (graph sh pa g)).
-  1: symmetry in H0; apply valid_parent in H0; auto.
-  eapply semax_ram_seq;
-    [subst RamFrame RamFrame0; unfold abbreviate;
-        repeat apply eexists_add_stats_cons; constructor
-    | semax_ram_call_body (sh, g, pa)
-    | semax_ram_after_call; intros [g' x']; simpl fst; simpl snd;
-      apply ram_extract_PROP; intros]. destruct H3 as [? ?].
-    unlocalize
-      (PROP ()
-       LOCAL (temp _p0 (pointer_val_val x'); temp _p (pointer_val_val pa);
-              temp _x (pointer_val_val x))
-       SEP (vertices_at sh (reachable g x) g'))
-    using [H3; H4]%RamAssu
-    binding [g'; x']%RamBind.
-  Grab Existential Variables.
-  Focus 3. {
-    Intros g' rt. forward. apply (exp_right g'). entailer !.
-    apply (exp_right rt). entailer !.
-  } Unfocus.
-  Focus 3. {
-    forward. apply (exp_right g). apply (exp_right x). entailer !.
-    assert (pa = x). {
-      hnf in H1. destruct pa, x; inversion H1; auto. simpl in H1. clear H5.
-      unfold sem_cmp_pp in H1. simpl in H1. destruct (eq_block b b0).
-      - destruct (Int.eq i i0) eqn:? .
-        + symmetry in Heqb1. apply binop_lemmas2.int_eq_true in Heqb1. subst; auto.
-        + simpl in H1. inversion H1.
-      - simpl in H1. inversion H1.
-    } subst pa. split; split; [|split| |]; auto.
-    - reflexivity.
-    - apply (uf_equiv_refl _  (liGraph g)).
-    - repeat intro; auto.
-    - apply uf_root_vgamma with (n := r); auto.
-  } Unfocus.
-  Focus 2. {
-    simplify_ramif. apply (@graph_ramify_aux_parent _ (sSGG_VST sh) _ g x r); auto.
-  } Unfocus.
-  unfold semax_ram.
-  forward.
-  assert (pa <> x). {
-    hnf in H1. destruct pa, x; inversion H1; [|intro; inversion H5..].
-    simpl in H1. clear H6. unfold sem_cmp_pp in H1.
-    simpl in H1. destruct (eq_block b b0).
-    - destruct (Int.eq i i0) eqn:? .
-      + simpl in H1. inversion H1.
-      + subst b0. apply int_eq_false_e in Heqb1. intro. inversion H5. auto.
-    - intro. inversion H5. auto.
-  } assert (weak_valid g' x') by (right; destruct H4; apply reachable_foot_valid in H4; auto).
-  assert (vvalid g' x) by (destruct H3 as [_ [[? _] _]]; rewrite <- H3; apply H).
+  forward_call (sh, g, pa). 1: symmetry in H0; apply valid_parent in H0; auto.
+  Intros vret. destruct vret as [g' root]. simpl in *. forward.
+  pose proof (true_Cne_neq _ _ H1).
+  assert (weak_valid g' root) by (right; destruct H3; apply reachable_foot_valid in H3; auto).
+  assert (vvalid g' x) by (destruct H2 as [_ [[? _] _]]; rewrite <- H2; apply H).
   assert ((vgamma g' x) = (r, pa)) by (apply (findS_preserves_vgamma g); auto).
-  assert (~ reachable g' x' x) by (destruct H4; apply (vgamma_not_reachable' _ _ r pa); auto).
+  assert (~ reachable g' root x) by (destruct H3; apply (vgamma_not_reachable' _ _ r pa); auto).
+  assert (vertices_at sh (vvalid (Graph_gen_redirect_parent g' x root H5 H6 H8)) (Graph_gen_redirect_parent g' x root H5 H6 H8) =
+          vertices_at sh (vvalid g') (Graph_gen_redirect_parent g' x root H5 H6 H8)). {
+    apply vertices_at_Same_set. unfold Ensembles.Same_set, Ensembles.Included, Ensembles.In. simpl. intuition. }
   localize
    (PROP  ()
-    LOCAL (temp _p (pointer_val_val x'); temp _x (pointer_val_val x))
+    LOCAL (temp _p (pointer_val_val root); temp _x (pointer_val_val x))
     SEP   (data_at sh node_type (Vint (Int.repr (Z.of_nat r)), pointer_val_val pa)
                    (pointer_val_val x))).
     eapply semax_ram_seq';
@@ -223,27 +197,70 @@ Proof.
       repeat apply eexists_add_stats_cons; constructor
     | store_tac 
     | abbreviate_semax_ram].
-    assert (force_val (sem_cast_neutral (pointer_val_val x')) = pointer_val_val x'). {
-      destruct x'; simpl; auto.
-    } rewrite H10. clear H10.
-    change (@field_at CompSpecs sh node_type [] (Vint (Int.repr (Z.of_nat r)), pointer_val_val x') (pointer_val_val x)) with
-    (@data_at CompSpecs sh node_type (Vint (Int.repr (Z.of_nat r)), pointer_val_val x') (pointer_val_val x)).
+    assert (force_val (sem_cast_neutral (pointer_val_val root)) = pointer_val_val root) by (destruct root; simpl; auto). rewrite H10. clear H10.
+    change (@field_at CompSpecs sh node_type [] (Vint (Int.repr (Z.of_nat r)), pointer_val_val root) (pointer_val_val x)) with
+        (@data_at CompSpecs sh node_type (Vint (Int.repr (Z.of_nat r)), pointer_val_val root) (pointer_val_val x)).
     unlocalize
       (PROP ()
-       LOCAL (temp _p (pointer_val_val x'); temp _x (pointer_val_val x))
-       SEP (vertices_at sh (reachable g x) (Graph_gen_redirect_parent g' x x' H6 H7 H9))).
+       LOCAL (temp _p (pointer_val_val root); temp _x (pointer_val_val x))
+       SEP (whole_graph sh (Graph_gen_redirect_parent g' x root H5 H6 H8))).
     Grab Existential Variables.
-    Focus 2. {
-      simplify_ramif. apply (@graph_gen_redirect_parent_ramify _ (sSGG_VST sh)); auto. destruct H4.
-      apply reachable_foot_valid in H4. intro. subst x'. apply (valid_not_null g' null H4). simpl. auto.
+    Focus 3. { Intros g' rt. forward. apply (exp_right g'). entailer !. apply (exp_right rt). entailer !. } Unfocus.
+    Focus 3. {
+      forward. apply (exp_right g). apply (exp_right x). entailer ! . apply false_Cne_eq in H1. subst pa. split; split; [|split| |]; auto.
+      - reflexivity.
+      - apply (uf_equiv_refl _  (liGraph g)).
+      - repeat intro; auto.
+      - apply uf_root_vgamma with (n := r); auto.
     } Unfocus.
-    unfold semax_ram.
-    forward. remember (Graph_gen_redirect_parent g' x x' H6 H7 H9) as g3. apply (exp_right g3).
-    apply (exp_right x'). entailer !. split.
-  - apply (graph_gen_redirect_parent_findS g g' x r pa x' H6 H7 H9); auto.
-  - simpl. apply (uf_root_gen_dst g' (liGraph g') x x x'); auto.
+    Focus 2. {
+      simplify_ramif. rewrite H9. apply (@graph_gen_redirect_parent_ramify _ (sSGG_VST sh)); auto. destruct H3.
+      apply reachable_foot_valid in H3. intro. subst root. apply (valid_not_null g' null H3). simpl. auto.
+    } Unfocus.
+    rewrite H9. unfold semax_ram. forward.
+    change (fun a : environ => (EX x0 : Graph, (EX x1 : pointer_val, (PROP (findS g x x0 /\ uf_root x0 x x1) LOCAL (temp _p (pointer_val_val x1); temp _x (pointer_val_val x))
+                                                                           SEP (vertices_at sh (vvalid x0) x0)) a))%logic) with
+        (EX x0 : Graph, (EX x1 : pointer_val, (PROP (findS g x x0 /\ uf_root x0 x x1) LOCAL (temp _p (pointer_val_val x1); temp _x (pointer_val_val x)) SEP
+                                                    (vertices_at sh (vvalid x0) x0)))). apply (exp_right (Graph_gen_redirect_parent g' x root H5 H6 H8)).
+    apply (exp_right root). rewrite H9. entailer !. split.
+  - apply (graph_gen_redirect_parent_findS g g' x r pa root H5 H6 H8); auto.
+  - simpl. apply (uf_root_gen_dst g' (liGraph g') x x root); auto.
     + apply (uf_root_edge _ (liGraph g') _ pa); auto. apply vgamma_not_dst with r; auto.
     + apply reachable_refl; auto.
-Qed. (* 85.7 secs *)
+Qed. (* 47.715 secs *)
 
 (* Print Assumptions body_find. *)
+
+Lemma true_Ceq_eq: forall x y, typed_true tint (force_val (sem_cmp_pp Ceq (pointer_val_val x) (pointer_val_val y))) -> x = y.
+Proof.
+  intros. hnf in H. destruct x, y; inversion H; auto. simpl in H. clear H1. unfold sem_cmp_pp in H. simpl in H. destruct (eq_block b b0).
+  - destruct (Int.eq i i0) eqn:? .
+    + symmetry in Heqb1. apply binop_lemmas2.int_eq_true in Heqb1. subst; auto.
+    + simpl in H. inversion H.
+  - simpl in H. inversion H.
+Qed.
+
+Lemma false_Ceq_neq: forall x y, typed_false tint (force_val (sem_cmp_pp Ceq (pointer_val_val x) (pointer_val_val y))) -> x <> y.
+Proof.
+  intros. hnf in H. destruct x, y; inversion H; [|intro; inversion H0..]. simpl in H. clear H1. unfold sem_cmp_pp in H. simpl in H. destruct (eq_block b b0).
+  - destruct (Int.eq i i0) eqn:? .
+    + simpl in H. inversion H.
+    + subst b0. apply int_eq_false_e in Heqb1. intro. inversion H0. auto.
+  - intro. inversion H0. auto.
+Qed.
+
+Lemma body_unionS: semax_body Vprog Gprog f_unionS unionS_spec.
+Proof.
+  start_function.
+  destruct H.
+  forward_call (sh, g, x). Intros vret. destruct vret as [g1 x_root]. simpl fst in *. simpl snd in *.
+  assert (vvalid g1 y) by (destruct H1 as [_ [[? _] _]]; rewrite <- H1; apply H0).
+  forward_call (sh, g1, y). Intros vret. destruct vret as [g2 y_root]. simpl fst in *. simpl snd in *.
+  forward_if_tac
+    (PROP ( )
+     LOCAL (temp _yRoot (pointer_val_val y_root); temp _xRoot (pointer_val_val x_root);
+     temp _x (pointer_val_val x); temp _y (pointer_val_val y))
+     SEP (vertices_at sh (vvalid g2) g2)). 1: apply ADMIT.
+  Focus 1. {
+    forward. apply (exp_right g2). entailer !; auto. apply true_Ceq_eq in H6. subst y_root.
+Abort.
